first commit

mergeSort.lean
@@ -1,6 +1,6 @@
 -- TODO remove the `partial`s and convince Lean that mergeSort terminates
 
-partial def merge [Ord A] (xs : List A) (ys : List A) : List A :=
+def merge [Ord A] (xs : List A) (ys : List A) : List A :=
   match xs, ys with
   | [], _ => ys
   | _, [] => xs
@@ -8,6 +8,7 @@ partial def merge [Ord A] (xs : List A) (ys : List A) : List A :=
     match Ord.compare x' y' with
     | .lt | .eq => x' :: merge xs' (y' :: ys')
     | .gt => y' :: merge (x'::xs') ys'
+termination_by merge xs ys => (xs, ys)
 
 def splitList (lst : List A) : (List A × List A) :=
   match lst with
@@ -16,14 +17,72 @@ def splitList (lst : List A) : (List A × List A) :=
     let (a, b) := splitList xs
     (x :: b, a)
 
-partial def mergeSort [Ord A] (xs : List A) : List A :=
+theorem succ_plus_1 (n : Nat):
+  (n + 1) = Nat.succ n := by simp
+
+theorem splitList_shorter (l : List A):
+  (splitList l).fst.length <= l.length /\
+  (splitList l).snd.length <= l.length := by
+  induction l
+  case nil =>
+    simp [splitList]
+  case cons x' l' IHl' =>
+    simp [splitList]
+    cases IHl'
+    constructor
+    case left =>
+      apply Nat.succ_le_succ
+      assumption
+    case right =>
+      apply Nat.le_succ_of_le
+      assumption
+
+theorem splitList_shorter_lt (l : List A) (Hlength : l.length >= 2) :
+  (splitList l).fst.length < l.length /\
+  (splitList l).snd.length < l.length := by
+    match l with
+    | a :: b :: l' =>
+      have Hshort : _ := splitList_shorter l'
+      cases Hshort
+      simp [splitList]
+      constructor
+      case left =>
+        apply Nat.succ_lt_succ
+        apply Nat.lt_succ_of_le
+        assumption
+      case right =>
+        apply Nat.succ_lt_succ
+        apply Nat.lt_succ_of_le
+        assumption
+
+theorem splitList_shorter_fst (l : List A) (Hlength : l.length >= 2):
+  (splitList l).fst.length < l.length := by
+  have H:_ := splitList_shorter_lt l Hlength
+  cases H
+  assumption
+
+theorem splitList_shorter_snd (l : List A) (Hlength : l.length >= 2):
+  (splitList l).snd.length < l.length := by
+  have H:_ := splitList_shorter_lt l Hlength
+  cases H
+  assumption
+
+def mergeSort [Ord A] (xs : List A) : List A :=
   if h : xs.length < 2 then
     match xs with
     | [] => []
     | [x] => [x]
   else
     let halves := splitList xs
+    have H: _ := Nat.ge_of_not_lt h
+    have: halves.fst.length < xs.length := by
+      apply splitList_shorter_fst
+      assumption
+    have: halves.snd.length < xs.length := by
+      apply splitList_shorter_snd
+      assumption
     merge (mergeSort halves.fst) (mergeSort halves.snd)
+termination_by mergeSort xs => xs.length
 
 def sorted (xs : List Nat) : Prop :=
   match xs with
@@ -31,7 +90,25 @@ def sorted (xs : List Nat) : Prop :=
   | _ :: [] => True
   | x :: y :: xs => x <= y /\ sorted (y :: xs)
 
+theorem merge_invariant (l1 l2 : List Nat):
+  sorted l1 -> sorted l2 -> sorted (merge l1 l2) := by sorry
+  -- intro H1 H2
+  -- induction l1
+  -- case nil =>
+  --   induction l2
+  --   case nil => simp [merge, sorted]
+  --   case cons =>
+  --     simp [merge]
+  --     assumption
+  -- case cons x1 l1' IHl1' =>
+  --   induction l2
+  --   case nil =>
+  --     simp [merge]
+  --     assumption
+  --   case cons x2 l2' IHl2' =>
+  --     simp [merge]
+  --     cases compare x1 x2
+
 theorem mergeSort_sorts (xs : List Nat) :
   sorted (mergeSort xs) := by
   sorry
-
